cequiv/approx_star.v
@@ -52,6 +52,8 @@ Require Import extensional_minus.
 Require Import extensional_abs.
 Require Import extensional_fresh.
 Require Import extensional_parallel.
+Require Import extensional_compseq1.
+Require Import extensional_compseq2.
 
 
 Theorem nuprl_extensional {p} : forall op, @extensional_op p op.
@@ -74,6 +76,8 @@ Proof.
     + Case "NFresh";    apply extensional_fresh.
     + Case "NTryCatch"; apply extensional_trycatch.
     + Case "NParallel"; apply extensional_parallel.
+    + Case "NCompSeq1"; apply extensional_comp_seq1.
+    + Case "NCompSeq2"; apply extensional_comp_seq2.
     + Case "NCompOp";   apply extensional_ncomp.
     + Case "NArithOp";  apply extensional_arith.
     + Case "NCanTest";  apply extensional_cantest.
