cequiv/extensional_compseq2.v
@@ -30,10 +30,11 @@
 
 *)
 
+
 Require Export approx_star0.
 
 
-Lemma extensional_apply {p} : extensional_op (@NCan p NApply).
+Lemma extensional_comp_seq2 {p} : forall nfo, extensional_op (@NCan p (NCompSeq2 nfo)).
 Proof.
   introv Hpra Hprt Hprt' Hcv Has Hi.
   applydup @compute_decompose_aux in Hcv; auto; exrepnd.
@@ -48,63 +49,46 @@ Proof.
   assert (skm <= k) by (subst; omega).
   apply reduces_atmost_S in XX; exrepnd.
   applydup @reduces_atmost_preserves_program in Hcv4; auto.
-  apply isprogram_apply_implies in Hcv6; exrepnd; subst; cpx.
+  apply isprogram_comp_seq2_implies_ex in Hcv6; unfold nobnd in *; exrepnd; subst; cpx.
 
   dorn Hcv0.
 
   - apply iscan_implies in Hcv0; repndors; exrepnd; subst.
 
     { csunf XX1; allsimpl.
-      apply compute_step_apply_success in XX1; repndors; exrepnd; subst; ginv.
+      apply compute_step_comp_seq2_success in XX1; exrepnd; repndors;
+        exrepnd; subst; unfold nobnd in *; ginv.
 
-      + (* destruct lhs for a bit so that the args of lambda show up*)
-        rename v into lamv.
-        rename b into lamb.
-        rename la into lamnt.
+      + apply reduces_in_atmost_k_steps_isvalue_implies in XX0; eauto 2 with slow; subst.
         apply no_change_after_value_ra with (k2:=k) in Hcv3; auto.
         duplicate Has.
         unfold lblift_sub in Has; repnd; allsimpl; cpx.
         repeat(approxrelbtd); show_hyps.
         make_red_val_like Hcv3 h.
         unfold extensional_op_ind in Hi.
-        apply Hi with (v := lamntr) in h; eauto; prove_isprogram.
+        apply Hi with (v := lar) in h; eauto; prove_isprogram.
         apply howe_lemma2 in h; exrepnd; auto; prove_isprogram.
         duplicate h1.
-        rename a into c.
         unfold approx_starbts, lblift_sub in h1; repnd; allsimpl; cpx.
-        repeat(approxrelbtd); show_hyps.
-        apply apply_bterm_approx_star_congr with
-        (lnt1:= [arg]) (lnt2:= [argr]) in h10bt; tcsp;
-        try (complete (intro xx; ginv));
-        [|prove_bin_rel_nterm; fail].
-        apply no_change_after_val_like with (k2 := k) in XX0; auto.
+        clear h1 h2.
         repnud h0.
 
         match goal with
-            [ |- approx_star _ _ (oterm (NCan ?no) _)] =>
-            let T := type of Has0 in
-            match T with
-              | lblift_sub _ _ (approx_star _) _ (_::?tr) =>
-                apply reduces_to_prinarg
-                with (lbt:= tr) (op:=no) in h1
-            end
+          [ |- approx_star _ _ (oterm (NCan ?no) _)] =>
+          let T := type of Has0 in
+          match T with
+          | lblift_sub _ _ (approx_star _) _ (_::?tr) =>
+            apply reduces_to_prinarg
+              with (lbt:= tr) (op:=no) in h1
+          end
         end. (* this will be used later in this proof *)
         pose proof (reduces_to_preserves_program _ _ _ h1 Hprt') as Hispr.
         apply reduces_atmost_preserves_program in Hcv4; auto; try omega.
 
-        make_red_val_like XX0 hh.
-
-        let T:= type of h10bt  in
-        match T with
-          | approx_star ?lib ?tl ?tr =>
-            assert (isprogram tl) by (apply (preserve_compute_step lib) with (t2:=tl) in Hcv4;sp);
-              assert(isprogram tr) by (apply (preserve_compute_step lib) with (t2:=tr) in Hispr;sp);
-              apply Hi with (v:=tr) in hh; auto;
-              apply approx_star_open_trans with (b:= tr); auto
-        end.
-        apply approx_implies_approx_open;
-          apply reduces_to_implies_approx_eauto;auto;
-          eapply reduces_to_if_split1; eauto.
+        apply approx_open_implies_approx_star.
+        apply reduces_to_implies_approx_open1; eauto 2 with slow.
+        eapply reduces_to_if_split1;[eauto|]; tcsp.
+        csunf; simpl; boolvar; autorewrite with slow; try omega; auto.
 
       + apply no_change_after_value_ra with (k2:=k) in Hcv3; auto.
         duplicate Has.
@@ -114,43 +98,40 @@ Proof.
         unfold extensional_op_ind in Hi.
         apply Hi with (v := lar) in h; eauto; prove_isprogram.
         apply howe_lemma2 in h; exrepnd; auto; prove_isprogram.
-        unfold approx_starbts, lblift_sub in h1; repnd; allsimpl; cpx.
-        clear h1.
+        duplicate h1.
         rename a into c.
+        unfold approx_starbts, lblift_sub in h1; repnd; allsimpl; cpx.
+        clear h1 h2.
+
         apply no_change_after_val_like with (k2 := k) in XX0; auto.
         repnud h0.
 
         match goal with
-            [ |- approx_star _ _ (oterm (NCan ?no) _)] =>
-            let T := type of Has0 in
-            match T with
-              | lblift_sub _ _ (approx_star _) _ (_::?tr) =>
-                apply reduces_to_prinarg
-                with (lbt:= tr) (op:=no) in h1
-            end
+          [ |- approx_star _ _ (oterm (NCan ?no) _)] =>
+          let T := type of Has0 in
+          match T with
+          | lblift_sub _ _ (approx_star _) _ (_::?tr) =>
+            apply reduces_to_prinarg
+              with (lbt:= tr) (op:=no) in h1
+          end
         end. (* this will be used later in this proof *)
         pose proof (reduces_to_preserves_program _ _ _ h1 Hprt') as Hispr.
         apply reduces_atmost_preserves_program in Hcv4; auto; try omega.
 
         make_red_val_like XX0 hh.
+        applydup @isprogram_comp_seq2_implies in Hprt'; repnd.
 
-        allrw <- @isprogram_apply_iff; repnd.
+        pose proof (Hi (mk_comp_seq2 (snoc l k0) i (mk_apply f (mk_nat (S (length l)))) f)
+                       c
+                       (mk_comp_seq2 (snoc l k0) i (mk_apply fr (mk_nat (S (length l)))) fr)) as q.
+        repeat (autodimp q hyp); eauto 2 with slow;
+          try (apply implies_isprogram_mk_comp_seq2; eauto 2 with slow).
+        { apply implies_approx_star_mk_comp_seq2; eauto 2 with slow. }
 
-        pose proof (Hi (mk_eapply (mk_choice_seq n) arg) c (mk_eapply (mk_choice_seq n) argr)) as q.
-        repeat (autodimp q hyp); try (apply isprogram_eapply); auto.
-        { apply approx_star_congruence3; try (apply isprogram_eapply); auto.
-          repeat (apply approx_starbts_cons; dands; eauto 3 with slow).
-          { unfold nobnd; prove_approx_star; auto.
-            apply approx_open_implies_approx_star.
-            apply approx_implies_approx_open; eauto 3 with slow. }
-          { unfold nobnd; prove_approx_star; auto. }
-        }
-
-        eapply approx_star_open_trans;[exact q|].
-        apply approx_implies_approx_open.
-        apply reduces_to_implies_approx_eauto;
-          allrw <- @isprogram_apply_iff; auto.
+        eapply approx_star_open_trans;[eauto|].
+        apply reduces_to_implies_approx_open1; eauto 2 with slow.
         eapply reduces_to_if_split1; eauto.
+        csunf; simpl; boolvar; autorewrite with slow in *; try omega; auto.
     }
 
   - apply isexc_implies in Hcv0; auto; exrepnd; subst.
@@ -172,7 +153,8 @@ Proof.
     apply approx_implies_approx_open.
     apply computes_to_exception_implies_approx; auto; prove_isprogram.
     allrw @computes_to_exception_as_reduces_to.
-    apply reduces_to_trans with (b := mk_apply (mk_exception a' e') a0r).
-    apply reduces_to_prinarg; auto.
+    destruct nfo as [ln kn].
+    apply reduces_to_trans with (b := mk_comp_seq2 ln kn (mk_exception a' e') t2r).
+    { apply reduces_to_prinarg; auto. }
     apply reduces_to_if_step; reflexivity.
 Qed.
